proof/gate.ec
@@ -2,17 +2,35 @@ require import Bitstring.
 require import Int.
 require import Map.
 require import Pair.
-
 require import Scheme.
 require import Dkc.
 
-cnst unit : unit.
+op lsb(b:bitstring) : bool = b.[0].
 
+op fst(x:'a*'b*'c) : 'a = let (a, b, c) = x in a.
+op snd(x:'a*'b*'c) : 'b = let (a, b, c) = x in b.
+op thi(x:'a*'b*'c) : 'c = let (a, b, c) = x in c.
+
+type token = Dkc.number.
+type tokens = (int*bool, token) map.
+
+op tweak(a:bool, b:bool) : bitstring = a::(b::(zeros (Scheme.k-2))).
+
+clone Scheme as Gate with
+  type funct = bool*bool*bool*bool,
+  type functG = token*token*token*token,
+  type input = bool*bool,
+  type output = bool,
+  type keyInput = token*token*token*token,
+  type keyOutput = unit,
+  type inputG = token*token,
+  type outputG = bool,
+  type random = tokens.
+
+(*
 theory Gate.
-  clone Scheme as Scheme.
-  export Scheme.
-
   type token = Dkc.number.
+  type tokens = (int*bool, Gate.token) map.
 
   type funct = bool*bool*bool*bool.
   type functG = token*token*token*token.
@@ -22,35 +40,34 @@ theory Gate.
   type keyOutput = unit.
   type inputG = token*token.
   type outputG = bool.
-
-  type tokens = (int*bool, Gate.token) map.
-
-  type query = (funct*input)*(funct*input).
-  type answer = functG*inputG*keyOutput.
-  
-  op tweak(a:bool, b:bool) : bitstring = a::(b::(zeros (k-2))).
   
   op eval(f:funct, i:input) : output =
     let (ff, ft, tf, tt) = f in
     let (i1, i2) = i in
-    if (((i1=false) && (i2=false))) then ff else
-    if (((i1=false) && (i2=true))) then ft else
-    if (((i1=true) && (i2=false))) then tf else
+    if !i1 && !i2 then ff else
+    if !i1 && i2 then ft else
+    if  i1 && !i2 then tf else
     tt.
 
   op enc(x:tokens, f:funct, x1:bool, x2:bool) : token =
-    Dkc.encode (tweak x1 x2) (proj x.[(1, x1)]) (proj x.[(2, x2)]) (proj x.[(3, eval f (x1,x2))]).
-  op garble(x:tokens, f:funct) : functG*keyInput*keyOutput =
+    let xx1 = (lsb (proj x.[(1, true)]) = x1) in
+    let xx2 = (lsb (proj x.[(2, true)]) = x2) in
+    Dkc.encode
+      (tweak x1 x2)
+      (proj x.[(1, xx1)])
+      (proj x.[(2, xx2)])
+      (proj x.[(3, eval f (xx1,xx2))]).
+  op _garble(x:tokens, f:funct) : functG*keyInput*keyOutput =
     (
       (enc x f false false, enc x f false true, enc x f true false, enc x f true true),
       (proj x.[(1, false)], proj x.[(1, true)], proj x.[(2, false)], proj x.[(2, true)]),
-      unit
+      tt
     ).
-  (*pred tokenCorrect(x:tokens) =
-    (to_array x.[(1, false)]).[0] != (to_array x.[(1, true)]).[0] &&
-    (to_array x.[(2, false)]).[0] != (to_array x.[(2, true)]).[0] &&
-    (to_array x.[(3, false)]).[0] == false &&
-    (to_array x.[(3, false)]).[0] == true.*)
+  pred tokenCorrect(x:tokens) =
+    (lsb (proj x.[(1, false)]) <> lsb (proj x.[(1, true)])) /\
+    (lsb (proj x.[(2, false)]) <> lsb (proj x.[(2, true)])) /\
+    (lsb (proj x.[(3, false)]) = false) /\
+    (lsb (proj x.[(3, true )]) = true).
 
   op encrypt(k:keyInput, i:input) : inputG =
     let (f1, t1, f2, t2) = k in
@@ -62,21 +79,70 @@ theory Gate.
 
   op evalG(g:functG, i:inputG) : outputG =
     let (ff, ft, tf, tt) = g in
-    let a = (fst i).[0] in
-    let b = (snd i).[0] in
+    let a = lsb (fst i) in
+    let b = lsb (snd i) in
     let t =
-      if (a = false) && (b = false) then ff else
-      if (a = false) && (b = true) then ft else
-      if (a = true) && (b = false) then tf else
+      if !a && !b then ff else
+      if !a &&  b then ft else
+      if  a && !b then tf else
       tt in
-    let u = Dkc.decode (tweak a b) (fst i) (snd i) t in
-    u.[0] (* C'est moche mais j'ai pas trouvé d'autre solution, c'est pas terrible*)
-    .
-    
+    lsb (Dkc.decode (tweak a b) (fst i) (snd i) t).
+
+  lemma oparg :
+    forall (f : 'a -> 'b),
+    forall (x : 'a),
+    forall (y : 'a),
+      (x = y) => (f x = f y).
+
   lemma inverse :
-    forall (f : funct) ,
     forall (i : input) ,
+    forall (f : funct) ,
     forall (x : tokens) ,
-      let (g, ki, ko) = garble x f in
-      eval f i = decrypt ko (evalG g (encrypt ki i)).
-end Gate.
+     let i1 = fst i in
+     let i2 = snd i in
+      tokenCorrect x =>
+      let temp = _garble x f in
+      let g = fst temp in
+      let ki = snd temp in
+      let ko = thi temp in
+      eval f (i1, i2) = decrypt ko (evalG g (encrypt ki (i1, i2)))
+  proof.
+
+  intros i f x i1 i2 tC g ki ko;
+  delta decrypt evalG encrypt g ki ko tC _garble Pair.fst Pair.snd fst snd.
+
+  case (i1).
+  case (i2).
+
+  simplify.
+  case (lsb (proj x.[(1, true)])).
+  simplify.
+  trivial.
+  simplify.
+  trivial.
+
+  simplify.
+  case (lsb (proj x.[(1, true)])).
+  simplify.
+  trivial.
+  simplify.
+  trivial.
+
+  case (i2).
+
+  simplify.
+  case (lsb (proj x.[(1, false)])).
+  simplify.
+  trivial.
+  simplify.
+  trivial.
+
+  simplify.
+  case (lsb (proj x.[(1, false)])).
+  simplify.
+  trivial.
+  simplify.
+  trivial.
+  save.
+
+end Gate.*)
