proof/garble.ec
@@ -3,7 +3,4 @@ require import Array.
 require import Bitstring.
 require import Scheme.
 
-theory Garble.
-  clone Scheme as Base.
-  export Base.
-end Gate.
+clone Scheme as Garble.
